verify/Compute.v
@@ -1,0 +1,261 @@
+(** * Compute: executable Turing machine model *)
+
+(** The model in [TM] uses coinductive, infinite streams, for which
+    equality is undecidable, and a step relation, which isn't
+    explicitly computable. This is nice for abstract reasoning,
+    but not directly usable for deciding Turing machines.
+    Here, we'll introduce a computable model, and prove
+    that corresponds to the abstract one. *)
+
+Set Warnings "-notation-overriden,-parsing,-deprecated-hint-without-locality".
+From Coq Require Import Bool.
+From Coq Require Import Lists.List. Import ListNotations.
+From Coq Require Import Lia.
+From BusyCoq Require Import LibTactics.
+From BusyCoq Require Import TM.
+Set Default Goal Selector "!".
+
+Lemma Cons_unfold : forall A (xs : Stream A),
+  xs = Cons (hd xs) (tl xs).
+Proof.
+  introv. destruct xs. reflexivity.
+Qed.
+
+Lemma const_unfold : forall T (x : T),
+  const x = Cons x (const x).
+Proof.
+  introv.
+  rewrite Cons_unfold at 1.
+  reflexivity.
+Qed.
+
+Lemma reflect_sym : forall A (x y : A) b,
+  reflect (x = y) b -> reflect (y = x) b.
+Proof.
+  introv H. destruct H; constructor; congruence.
+Qed.
+
+Definition ctape (S : Type) : Type := list S * S * list S.
+
+Section TMs.
+  Context {Q Sym : Type}.
+  Variable q0 : Q.
+  Variable s0 : Sym.
+  Variable tm : TM Q Sym.
+
+  Variable eqb_sym : Sym -> Sym -> bool.
+  Variable eqb_sym_spec : forall a b, reflect (a = b) (eqb_sym a b).
+
+  Variable eqb_q : Q -> Q -> bool.
+  Variable eqb_q_spec : forall a b, reflect (a = b) (eqb_q a b).
+
+  Notation tape := (tape Sym).
+  Notation ctape := (ctape Sym).
+  Notation c0 := (c0 q0 s0).
+
+Fixpoint lift_side (xs : list Sym) : Stream Sym :=
+  match xs with
+  | [] => const s0
+  | x :: xs => Cons x (lift_side xs)
+  end.
+
+Definition lift_tape (t : ctape) : tape :=
+  match t with (l, s, r) => (lift_side l, s, lift_side r) end.
+
+Definition lift (c : Q * ctape) : Q * tape :=
+  match c with (q, t) => (q, lift_tape t) end.
+
+Fixpoint empty_side (xs : list Sym) : bool :=
+  match xs with
+  | x :: xs => eqb_sym x s0 && empty_side xs
+  | [] => true
+  end.
+
+Lemma empty_side_spec : forall xs,
+  reflect (lift_side xs = const s0) (empty_side xs).
+Proof.
+  induction xs.
+  - apply ReflectT. reflexivity.
+  - simpl.
+    destruct (eqb_sym_spec a s0) as [E | Hneq].
+    + subst a.
+      inverts IHxs as Elift Eempty.
+      * apply ReflectT. rewrite Elift, <- const_unfold. reflexivity.
+      * apply ReflectF. rewrite const_unfold. congruence.
+    + apply ReflectF. rewrite const_unfold. congruence.
+Qed.
+
+Fixpoint eqb_side (xs ys : list Sym) : bool :=
+  match xs with
+  | x :: xs' =>
+    match ys with
+    | y :: ys' => eqb_sym x y && eqb_side xs' ys'
+    | [] => empty_side xs
+    end
+  | [] => empty_side ys
+  end.
+
+Lemma eqb_side_spec : forall xs ys,
+  reflect (lift_side xs = lift_side ys) (eqb_side xs ys).
+Proof.
+  induction xs; intros ys.
+  - simpl. apply reflect_sym, empty_side_spec.
+  - destruct ys as [| y ys].
+    + apply empty_side_spec.
+    + simpl.
+      destruct (eqb_sym_spec a y) as [E | Hneq].
+      * subst a. simpl.
+        destruct (IHxs ys) as [E | Hneq]; constructor; congruence.
+      * apply ReflectF. congruence.
+Qed.
+
+Definition eqb_tape (t t' : ctape) : bool :=
+  match t, t' with
+  | (l, s, r), (l', s', r') =>
+    eqb_side l l' && eqb_sym s s' && eqb_side r r'
+  end.
+
+Lemma eqb_tape_spec : forall t t',
+  reflect (lift_tape t = lift_tape t') (eqb_tape t t').
+Proof.
+  intros [[l s] r] [[l' s'] r']. simpl.
+  apply iff_reflect.
+  repeat rewrite andb_true_iff.
+  rewrite <- (reflect_iff _ _ (eqb_side_spec l l')).
+  rewrite <- (reflect_iff _ _ (eqb_sym_spec  s s')).
+  rewrite <- (reflect_iff _ _ (eqb_side_spec r r')).
+  repeat split; try (inverts H; auto).
+  intros [[H1 H2] H3]. congruence.
+Qed.
+
+Definition eqb (c c' : Q * ctape) : bool :=
+  match c, c' with
+  | q; t, q'; t' => eqb_q q q' && eqb_tape t t'
+  end.
+
+Lemma eqb_spec : forall c c',
+  reflect (lift c = lift c') (eqb c c').
+Proof.
+  intros [q t] [q' t']. simpl.
+  apply iff_reflect. rewrite andb_true_iff.
+  rewrite <- (reflect_iff _ _ (eqb_q_spec q q')).
+  rewrite <- (reflect_iff _ _ (eqb_tape_spec t t')).
+  repeat split; try (inverts H; auto).
+  intros [H1 H2]. congruence.
+Qed.
+
+Definition left (t : ctape) : ctape :=
+  match t with
+  | ([], s, r) => ([], s0, s :: r)
+  | (s' :: l, s, r) => (l, s', s :: r)
+  end.
+
+Definition right (t : ctape) : ctape :=
+  match t with
+  | (l, s, []) => (s :: l, s0, [])
+  | (l, s, s' :: r) => (s :: l, s', r)
+  end.
+
+Arguments left t : simpl never.
+Arguments right t : simpl never.
+
+Lemma lift_left : forall t, lift_tape (left t) = move_left (lift_tape t).
+Proof.
+  intros [[[| s' l] s] r]; reflexivity.
+Qed.
+
+Lemma lift_right : forall t, lift_tape (right t) = move_right (lift_tape t).
+Proof.
+  intros [[l s] [| s' r]]; reflexivity.
+Qed.
+
+Definition cstep (c : Q * ctape) : option (Q * ctape) :=
+  match c with
+  | q; l {{s}} r =>
+    match tm (q, s) with
+    | None => None
+    | Some (s', L, q') => Some (q'; left  (l {{s'}} r))
+    | Some (s', R, q') => Some (q'; right (l {{s'}} r))
+    end
+  end.
+
+Lemma cstep_halting : forall c,
+  cstep c = None -> halting tm (lift c).
+Proof.
+  intros [q [[l s] r]] H. unfold halting.
+  simpl. simpl in H.
+  destruct (tm (q; s)) as [[[s' []] q'] |]; try discriminate.
+  reflexivity.
+Qed.
+
+Lemma cstep_some : forall c c',
+  cstep c = Some c' ->
+  lift c -[ tm ]-> lift c'.
+Proof.
+  introv H.
+  destruct c as [q [[l s] r]].
+  simpl. simpl in H.
+  destruct (tm (q; s)) as [[[s' []] q1] |] eqn:E; inverts H as; simpl.
+  - rewrite lift_left. apply step_left. assumption.
+  - rewrite lift_right. apply step_right. assumption.
+Qed.
+
+Fixpoint cmultistep (n : nat) (c : Q * ctape) : option (Q * ctape) :=
+  match n with
+  | 0 => Some c
+  | S n' =>
+    match cstep c with
+    | Some c' => cmultistep n' c'
+    | None => None
+    end
+  end.
+
+Lemma cmultistep_some : forall n c c',
+  cmultistep n c = Some c' ->
+  lift c -[ tm ]->* n / lift c'.
+Proof.
+  induction n; introv H; simpl in H.
+  - inverts H. apply multistep_0.
+  - destruct (cstep c) as [c1 |] eqn:E.
+    + apply IHn in H. apply cstep_some in E.
+      eapply multistep_S; eassumption.
+    + discriminate.
+Qed.
+
+Lemma cmultistep_halts_in : forall n c,
+  cmultistep n c = None ->
+  exists n', n' < n /\ halts_in tm (lift c) n'.
+Proof.
+  induction n; introv H.
+  - discriminate.
+  - simpl in H. destruct (cstep c) as [c1 |] eqn:E.
+    + apply IHn in H. apply cstep_some in E.
+      destruct H as [n' [Hlt [ch [Hrun Hhalting]]]].
+      exists (S n'). split.
+      * lia.
+      * exists ch. split.
+        ** eapply multistep_S; eassumption.
+        ** assumption.
+    + apply cstep_halting in E. exists 0. split.
+      * lia.
+      * exists (lift c). split.
+        ** apply multistep_0.
+        ** assumption.
+Qed.
+
+Corollary cmultistep_halts : forall n c,
+  cmultistep n c = None ->
+  halts tm (lift c).
+Proof.
+  introv H.
+  apply cmultistep_halts_in in H.
+  destruct H as [n' [_ H]].
+  exists n'. exact H.
+Qed.
+
+Definition starting : Q * ctape := q0; [] {{s0}} [].
+
+Lemma lift_starting : lift starting = c0.
+Proof. reflexivity. Qed.
+
+End TMs.
