verify/Cyclers.v
@@ -1,0 +1,113 @@
+(** * Cyclers *)
+
+Set Warnings "-notation-overriden,-parsing,-deprecated-hint-without-locality".
+From Coq Require Import Bool.Bool.
+From Coq Require Import Arith.Arith.
+From Coq Require Import Lia.
+From Coq Require Import Lists.List. Import ListNotations.
+From Coq Require Extraction. Require Import ExtrOcamlBasic.
+From BusyCoq Require Import LibTactics.
+From BusyCoq Require Import TM.
+From BusyCoq Require Import Compute.
+Set Default Goal Selector "!".
+
+Section TMs.
+  Context {Q Sym : Type}.
+  Variable q0 : Q.
+  Variable s0 : Sym.
+
+  Variable eqb_sym : Sym -> Sym -> bool.
+  Variable eqb_sym_spec : forall a b, reflect (a = b) (eqb_sym a b).
+
+  Variable eqb_q : Q -> Q -> bool.
+  Variable eqb_q_spec : forall a b, reflect (a = b) (eqb_q a b).
+
+  Notation TM := (TM Q Sym).
+  Notation tape := (tape Sym).
+  Notation ctape := (ctape Sym).
+  Notation c0 := (c0 q0 s0).
+  Notation starting := (starting q0 s0).
+  Notation cmultistep := (cmultistep s0).
+  Notation eqb := (eqb s0 eqb_sym eqb_q).
+  Notation lift := (lift s0).
+
+Definition verify_cycler (tm : TM) (n k : nat) : bool :=
+  match cmultistep tm n starting with
+  | Some c =>
+    match cmultistep tm k c with
+    | Some c' => (0 <? k) && eqb c c'
+    | None => false
+    end
+  | None => false
+  end.
+
+Lemma eventually_exceeds :
+  forall a d h, d > 0 ->
+  exists k, a + k * d > h.
+Proof.
+  introv H.
+  induction h.
+  - exists 1. lia.
+  - destruct IHh as [k IH].
+    exists (S k). lia.
+Qed.
+
+Lemma cycle_chain :
+  forall (tm : TM) c n k,
+  c -[ tm ]->* k / c ->
+  c -[ tm ]->* (n * k) / c.
+Proof.
+  introv H.
+  induction n.
+  - apply multistep_0.
+  - simpl. eapply multistep_trans; eassumption.
+Qed.
+
+Lemma cycle_nonhalting :
+  forall (tm : TM) c1 c2 n k,
+  k > 0 ->
+  c1 -[ tm ]->* n / c2 ->
+  c2 -[ tm ]->* k / c2 ->
+  ~ halts tm c1.
+Proof.
+  introv Hgt0 Hn Hk [h [ch [Hh Hhalting]]].
+  destruct (eventually_exceeds n k h Hgt0) as [r Hr].
+  assert (Hreach : c1 -[ tm ]->* (n + r * k) / c2).
+  { eapply multistep_trans.
+    - exact Hn.
+    - apply cycle_chain. exact Hk. }
+  assert (Hsplit : exists w, w > 0 /\ h + w = n + r * k).
+  { exists (n + r * k - h). lia. }
+  destruct Hsplit as [w [Hwgt0 Ehw]].
+  rewrite <- Ehw in Hreach.
+  apply rewind_split in Hreach.
+  destruct Hreach as [ch' [Hh' Hw]].
+  assert (Ech' : ch = ch').
+  { eapply multistep_deterministic; eassumption. }
+  rewrite <- Ech' in Hw.
+  eapply halting_no_multistep in Hhalting.
+  - apply Hhalting in Hw. contradiction.
+  - assumption.
+Qed.
+
+Theorem verify_cycler_correct : forall tm n k,
+  verify_cycler tm n k = true -> ~ halts tm c0.
+Proof.
+  introv H. unfold verify_cycler in H.
+  destruct (cmultistep tm n starting) as [c |] eqn:E; try discriminate.
+  destruct (cmultistep tm k c) as [c' |] eqn:E'; try discriminate.
+  rewrite andb_true_iff, Nat.ltb_lt in H. destruct H as [Hgt0 H].
+  assert (Hs : reflect (lift c = lift c') (eqb c c'))
+    by (apply eqb_spec; assumption).
+  inverts Hs as Elift Eeqb; try congruence.
+
+  apply cmultistep_some in E, E'.
+  rewrite lift_starting in E.
+  rewrite <- Elift in E'.
+  eapply cycle_nonhalting; eassumption.
+Qed.
+
+End TMs.
+
+Extraction Language OCaml.
+Extraction "cyclers.ml" verify_cycler.
